

# Tarea 1

Simplifica

$$\begin{aligned}
 30. & [(\sim p \vee q) \wedge (\sim q \rightarrow p)] \rightarrow (p \wedge \sim q) \\
 & [(\sim p \vee q) \wedge (q \vee p)] \rightarrow (p \wedge \sim q) \\
 & [q \vee (p \wedge \sim p)] \rightarrow (p \wedge \sim q) \\
 & (q \vee F) \rightarrow (p \wedge \sim q) \\
 & \sim q \vee (p \wedge \sim q) \\
 & \sim q
 \end{aligned}$$

// (L. implicación y L. neg)  
 // (L. distributiva)  
 // (L. Negación)  
 // (L. implicación, L. identidad)  
 // (L. absorción)

$$\begin{aligned}
 35. & (\sim p \vee q) \rightarrow [p \wedge \sim(p \wedge \sim q)] \\
 & \sim(\sim p \vee q) \vee [p \wedge \sim(p \wedge \sim q)] \\
 & (p \wedge \sim q) \vee [(p \wedge \sim p) \vee (p \wedge q)] \\
 & (p \wedge \sim q) \vee [F \vee (p \wedge q)] \\
 & (p \wedge \sim q) \vee (p \wedge q) \\
 & (p \wedge \sim q) \vee (p \wedge q) \\
 & p \wedge (q \vee \sim q) \\
 & p \wedge V \\
 & p
 \end{aligned}$$

// (L. implicación y L. Morgan)  
 // (L. Morgan y L. distributiva)  
 // (L. negación)  
 // (L. identidad)  
 // (L. distributiva)  
 // (L. negación)  
 // (L. identidad)

$$\begin{aligned}
 40. & [p \rightarrow (p \wedge \sim q)] \wedge [(p \vee q) \rightarrow p] \\
 & [\sim p \vee (p \wedge \sim q)] \wedge [\sim(p \vee q) \vee p] \\
 & [(\sim p \vee p) \wedge (\sim p \vee \sim q)] \wedge [(\sim p \wedge \sim q) \vee p] \\
 & [V \wedge (\sim p \vee \sim q)] \wedge [(p \vee \sim p) \wedge (p \vee \sim q)] \\
 & (\sim p \vee \sim q) \wedge [V \wedge (p \vee \sim q)] \\
 & (\sim p \vee \sim q) \wedge (p \vee \sim q) \\
 & \sim q \vee (p \wedge \sim p) \\
 & \sim q \vee F \\
 & \sim q
 \end{aligned}$$

// (L. implicación)  
 // (L. Morgan y L. distributiva)  
 // (L. neg y L. distributiva)  
 // (L. identidad y L. neg)  
 // (L. identidad)  
 // (L. distributiva)  
 // (L. neg)  
 // (L. identidad)

$$45. [(p \wedge \sim q) \vee (p \wedge \sim r)] \wedge [(p \vee \sim r) \wedge \sim p]$$

$$\begin{aligned}
45. & [(p \wedge \sim q) \vee (q \wedge r)] \wedge [(q \vee r) \wedge \sim r] \\
& [(p \wedge \sim q) \vee (q \wedge r)] \wedge [(\sim r \wedge q) \vee (\sim r \wedge r)] \\
& [(p \wedge \sim q) \vee (q \wedge r)] \wedge [(\sim r \wedge q) \vee \text{F}] \\
& [(p \wedge \sim q) \vee (q \wedge r)] \wedge (\sim r \wedge q) \\
& [(\sim r \wedge q) \wedge (p \wedge \sim q)] \vee [(\sim r \wedge q) \wedge (q \wedge r)] \\
& [(\sim r \wedge q) \wedge (p \wedge \sim q)] \vee [(\sim r \wedge r) \wedge (q \wedge q)] \\
& [(\sim r \wedge q) \wedge (p \wedge \sim q)] \vee [\text{F} \wedge (q \wedge q)] \\
& \text{F} \vee \text{F} \\
& \text{F}
\end{aligned}$$

// (L. distributiva)  
 // (L. neg)  
 // (L. identidad)  
 // (L. distributiva)  
 // (L. conmutativa)  
 // (L. neg)  
 // (L. neg)

Simplifica

$$\begin{aligned}
1. & [(\sim q \rightarrow r) \wedge \sim(q \wedge \sim r)] \rightarrow [(r \rightarrow p) \wedge (p \rightarrow \sim r)] \\
& [(q \vee r) \wedge (\sim q \vee r)] \rightarrow [(\sim r \vee p) \wedge (\sim p \vee \sim r)] \\
& [r \vee (q \wedge \sim q)] \rightarrow [\sim r \vee (p \wedge \sim p)] \\
& (r \vee \text{F}) \rightarrow (\sim r \vee \text{F}) \\
& r \vee \sim r \\
& \text{T}
\end{aligned}$$

// (L. idempotencia y L. Morgan)  
 // (L. distributiva)  
 // (L. neg)  
 // (L. identidad) (L. implicación)  
 // (L. idempotencia)



$$\begin{aligned}
 2. & [(r \rightarrow p) \rightarrow (p \wedge r)] \rightarrow [(r \vee q) \rightarrow (\sim r \wedge q)] \\
 & [(\sim r \vee p) \rightarrow (p \wedge r)] \rightarrow [\sim(r \vee q) \vee (\sim r \wedge q)] \\
 & \sim[\sim(\sim r \vee p) \vee (p \wedge r)] \vee [(\sim r \wedge \sim q) \vee (\sim r \wedge q)] \\
 & \sim[(\sim r \wedge p) \vee (p \wedge r)] \vee [\sim r \wedge (\sim q \vee q)] \\
 & \sim[r \wedge (\sim p \vee p)] \vee [\sim r \wedge V] \\
 & \sim(r \wedge V) \vee \sim r \\
 & \sim r \vee \sim r \\
 & \underline{\sim r}
 \end{aligned}$$

// (L. implicación)  
 // (L. implicación y L. Morgan)  
 // (L. Morgan y distributiva)  
 // (L. neg y distributiva)  
 // (L. identidad y neg)  
 // (L. identidad)  
 // (L. idempotencia)

Demuestra

$$3. [(p \rightarrow r) \wedge \sim p] \vee [(p \vee q) \rightarrow r] \equiv \sim p \vee r$$

$$\begin{aligned}
 & [(\sim p \vee r) \wedge \sim p] \vee [\sim(p \vee q) \vee r] \\
 & \sim p \vee [(\sim p \wedge \sim q) \vee r] \\
 & [\sim p \vee (\sim p \wedge \sim q)] \vee r \\
 & \sim p \vee r \\
 & \underline{\sim p \vee r}
 \end{aligned}$$

// (L. implicación)  
 // (L. absorción)  
 // (L. asociativa)  
 // (L. absorción)